DeBruijnSSA/BinSyntax/Rewrite/Region/Structural.lean
@@ -97,6 +97,11 @@ theorem Eqv.vsubst_liftn₂_packed {Γ Δ Δ' : Ctx α ε} {R : LCtx α} {r : Eq
   : r.packed.vsubst (σ.liftn₂ (le_refl _) (le_refl V)) = r.packed (L := L) (Δ := _::Δ') := by
   simp [<-Term.Subst.Eqv.lift_lift]
 
+@[simp]
+theorem Eqv.lwk1_packed {Γ Δ : Ctx α ε} {R : LCtx α} {r : Eqv φ Γ R}
+  : r.packed.lwk1 (inserted := inserted) = r.packed (L := _::L)  (Δ := Δ) := by
+  rw [packed_def', lwk1_packed_out, <-packed_def']
+
 open Term.Eqv
 
 theorem Eqv.packed_br {Γ : Ctx α ε} {L : LCtx α}
@@ -157,12 +162,13 @@ theorem Eqv.packed_cfg_split {Γ : Ctx α ε} {L R : LCtx α} {β : Eqv φ Γ (R
       (ret Term.Eqv.split ;; _ ⋊ β.packed.unpacked_app_out)
       (ret Term.Eqv.split ⋉ _ ;; assoc
         ;; _ ⋊ (ret Term.Eqv.distl_pack
-          ;; pack_coprod (λi => acast R.get_dist
-            ;; (G (i.cast R.length_dist)).packed.unpacked_app_out))) := by
+          ;; (pack_coprod (λi => acast R.get_dist
+            ;; (G (i.cast R.length_dist)).packed)).unpacked_app_out)) := by
   rw [packed, packed_out_cfg_letc, packed_in_letc_split]
   congr 3
   · rw [packed_in_unpacked_app_out, <-packed]
-  · rw [packed_in_pack_coprod_arr]; congr; funext i; rw [packed_in_unpacked_app_out, <-packed]
+  · rw [packed_in_pack_coprod_arr, unpacked_app_out_pack_coprod]
+    congr; funext i; rw [packed_in_unpacked_app_out, <-packed, unpacked_app_out_seq, lwk1_acast]
 
 theorem Eqv.packed_cfg_split_vwk1 {Γ : Ctx α ε} {L R : LCtx α} {β : Eqv φ Γ (R ++ L)} {G}
   : (cfg R β G).packed (Δ := Δ)
@@ -170,8 +176,8 @@ theorem Eqv.packed_cfg_split_vwk1 {Γ : Ctx α ε} {L R : LCtx α} {β : Eqv φ 
       (ret Term.Eqv.split ;; _ ⋊ β.packed.unpacked_app_out)
       (ret Term.Eqv.split ⋉ _ ;; assoc
         ;; _ ⋊ (ret Term.Eqv.distl_pack
-          ;; pack_coprod (λi => acast R.get_dist
-            ;; (G (i.cast R.length_dist)).packed.unpacked_app_out))).vwk1 := by
+          ;; (pack_coprod (λi => acast R.get_dist
+            ;; (G (i.cast R.length_dist)).packed)).unpacked_app_out)).vwk1 := by
   rw [packed_cfg_split]
   simp only [List.get_eq_getElem, Fin.coe_cast, vwk1_seq, vwk1_ltimes, vwk1_br, wk1_split,
     vwk1_rtimes, wk1_distl_pack, vwk1_pack_coprod, vwk1_acast, vwk1_unpacked_app_out, vwk1_packed]
